Implemented float comparisons (no branching yet, and no negation)

mppa_k1c/PostpassSchedulingOracle.ml
@@ -55,6 +55,7 @@ let arith_rr_str = function
 let arith_rrr_str = function
   | Pcompw it -> "Pcompw"
   | Pcompl it -> "Pcompl"
+  | Pfcompw ft -> "Pfcompw"
   | Paddw -> "Paddw"
   | Psubw -> "Psubw"
   | Pmulw -> "Pmulw"
@@ -305,6 +306,10 @@ let alu_lite : int array = let resmap = fun r -> match r with
   | "ISSUE" -> 1 | "TINY" -> 1 | "LITE" -> 1 |  _ -> 0 
   in Array.of_list (List.map resmap resource_names)
 
+let alu_lite_x : int array = let resmap = fun r -> match r with 
+  | "ISSUE" -> 2 | "TINY" -> 1 | "LITE" -> 1 |  _ -> 0 
+  in Array.of_list (List.map resmap resource_names)
+
 let alu_full : int array = let resmap = fun r -> match r with
   | "ISSUE" -> 1 | "TINY" -> 1 | "LITE" -> 1 | "ALU" -> 1 | _ -> 0
   in Array.of_list (List.map resmap resource_names)
@@ -373,6 +378,7 @@ type real_instruction =
   | Fabsd | Fabsw | Fnegw | Fnegd
   | Faddd | Faddw | Fsbfd | Fsbfw | Fmuld | Fmulw
   | Fnarrowdw | Fwidenlwd | Floatwz | Floatuwz | Floatdz | Floatudz | Fixedwz | Fixeduwz | Fixeddz | Fixedudz
+  | Fcompw
 
 let ab_inst_to_real = function
   | "Paddw" | "Paddiw" | "Pcvtl2w" -> Addw
@@ -381,6 +387,7 @@ let ab_inst_to_real = function
   | "Pandl" | "Pandil" -> Andd
   | "Pcompw" | "Pcompiw" -> Compw
   | "Pcompl" | "Pcompil" -> Compd
+  | "Pfcompw" -> Fcompw
   | "Pmulw" -> Mulw
   | "Pmull" -> Muld
   | "Porw" | "Poriw" -> Orw
@@ -470,6 +477,9 @@ let rec_to_usage r =
   | Compd -> (match encoding with None | Some U6 | Some S10 -> alu_tiny
                                 | Some U27L5 | Some U27L10 -> alu_tiny_x
                                 | Some E27U27L10 -> alu_tiny_y)
+  | Fcompw -> (match encoding with None -> alu_lite
+                                | Some U6 | Some S10 | Some U27L5 -> alu_lite_x
+                                | _ -> raise InvalidEncoding)
   | Make -> (match encoding with Some U6 | Some S10 -> alu_tiny 
                           | Some U27L5 | Some U27L10 -> alu_tiny_x 
                           | Some E27U27L10 -> alu_tiny_y 
@@ -502,7 +512,7 @@ let real_inst_to_latency = function
   | Nop -> 0 (* Only goes through ID *)
   | Addw | Andw | Compw | Orw | Sbfw | Sraw | Srlw | Sllw | Xorw
   | Addd | Andd | Compd | Ord | Sbfd | Srad | Srld | Slld | Xord | Make
-  | Sxwd | Zxwd
+  | Sxwd | Zxwd | Fcompw
         -> 1
   | Floatwz | Floatuwz | Fixeduwz | Fixedwz | Floatdz | Floatudz | Fixeddz | Fixedudz -> 4
   | Mulw | Muld -> 2 (* FIXME - WORST CASE. If it's S10 then it's only 1 *)
